Types/Utils.lean
@@ -4,3 +4,113 @@ instance : HAdd NumLit Nat NumLit where
 
 def Nat.split : ∀ n, ∃ a b : Nat, n = a + b := fun n => ⟨n, 0, rfl⟩
 
+namespace List
+
+inductive MemT : A → List A → Type
+  | hd {a as} : MemT a (a :: as)
+  | tl {bs a b} : MemT a bs → MemT a (b :: bs)
+
+namespace MemT
+
+def shift {A a} {l₁}
+    : {l₂ : List A}
+    → l₁.MemT a
+    → (l₂ ++ l₁).MemT a
+  | [], h => h
+  | _ :: _, h => .tl (shift h)
+
+def sandwitch_shift {A a l₁}
+    : {l l₂ : List A}
+    → (l ++ l₁).MemT a
+    → (l ++ (l₂ ++ l₁)).MemT a
+  | [], _, h => h.shift
+  | _ :: _, _, .hd => .hd
+  | _ :: _, _, .tl v => .tl v.sandwitch_shift
+
+def remove
+    {A v}
+    : {l : List A}
+    → l.MemT v
+    → List A 
+  | _ :: t, .hd => t
+  | h :: _, .tl h' => h :: remove h'
+
+def map {f : A → B}
+    : {l : List A}
+    → l.MemT v
+    → (l.map f).MemT (f v)
+  | _ :: _, .hd => .hd
+  | _ :: _, .tl h => .tl h.map
+
+/- def mapo {f : A → B} -/
+/-     : {l : List A} -/
+/-     → l.MemT v -/
+/-     → (l.map f).MemT (f v) -/
+
+end List.MemT
+
+inductive HList {A} (f : A → Type _) : List A → Type _
+  | nil : HList f []
+  | cons {hd tl} : f hd → HList f tl → HList f (hd :: tl)
+
+namespace HList
+
+def get : {Γ : _} → List.MemT (A := A) t Γ → HList f Γ → f t
+  | _ :: _, .hd, .cons h _ => h
+  | _ :: _, .tl v, .cons _ tl => tl.get v
+
+def map {f g} (h : ∀ {v}, f v → g v) : HList f Γ → HList g Γ
+  | .nil => .nil
+  | .cons hd tl => .cons (h hd) <| tl.map h
+
+@[simp]
+theorem get_map {f g : A → Type _}
+    {h : ∀ {v}, f v → g v}
+    : {ls : HList f Γ} → (i : List.MemT a Γ) → (ls.map h).get i = h (ls.get i)
+  | .cons _ _, .hd => rfl
+  | .cons hd tl, .tl h' => by
+    change get h' (map h tl) = h (tl.get h')
+    exact get_map _
+
+def map' {Γm : A → B} {f g} (h : ∀ {v}, f v → g (Γm v)) : HList f Γ → HList g (Γ.map Γm)
+  | .nil => .nil
+  | .cons hd tl => .cons (h hd) <| tl.map' h
+
+/- @[simp] -/
+/- theorem get_map' -/
+/-     {Γm : A → B} {f : A → Type _} {g : B → _} (h : ∀ {v}, f v → g (Γm v)) -/
+/-     : {ls : HList f Γ} → (i : List.MemT a _) → (ls.map' h).get i = _ -/
+/-   | .cons _ _, .hd => rfl -/
+/-   | .cons hd tl, .tl h' => by  -/
+/-     change get h' (map h tl) = h (tl.get h') -/
+/-     exact get_map _ -/
+
+end HList
+
+inductive Vec (T : Type u) : Nat → Type u
+  | nil : Vec T 0
+  | cons : T → Vec T n → Vec T (n + 1)
+
+namespace Vec
+
+def get : Vec T n → Fin n → T
+  | .cons h _, ⟨0, _⟩ => h
+  | .cons _ tl, ⟨n+1, h'⟩ => tl.get ⟨n, Nat.succ_lt_succ_iff.mp h'⟩
+
+@[simp]
+theorem get_zero {h} {t : Vec T n} : (Vec.cons h t).get (0 : Fin (n+1)) = h := rfl
+@[simp]
+theorem get_succ {h} {t : Vec T n} {i : Fin n} : (Vec.cons h t).get (Fin.succ i) = t.get i := rfl
+
+def map (f : A → B) : Vec A n → Vec B n
+  | .nil => .nil
+  | .cons hd tl => .cons (f hd) <| tl.map f
+
+@[simp]
+theorem get_map (f : A → B)
+    : {ls : Vec A n} → (i : Fin n) → (ls.map f).get i = f (ls.get i)
+  | .cons _ _, ⟨0, _⟩ => rfl
+  | .cons _ _, ⟨n+1, h'⟩ => get_map f ⟨n, Nat.succ_lt_succ_iff.mp h'⟩
+
+end Vec
+
