Types/DataFun/Stx.lean
@@ -1,0 +1,99 @@
+import Types.Utils
+import Types.DataFun.Ty
+
+namespace DF
+
+def dize : List ModalType → List ModalType :=
+  List.filter ModalType.IsDisc
+
+theorem dize_app {A B : List ModalType} : dize (A ++ B) = dize A ++ dize B := by
+  simp [dize]
+
+inductive Stx : List ModalType → Ty → Type
+  | var : List.MemT v Γ → Stx Γ v.out
+
+  | unit : Stx Γ .unit
+  | prod : Stx Γ A → Stx Γ B → Stx Γ (.prod A B)
+  | fst : Stx Γ (.prod A B) → Stx Γ A
+  | snd : Stx Γ (.prod A B) → Stx Γ B
+
+  | inl : Stx Γ A → Stx Γ (.cop A B)
+  | inr : Stx Γ B → Stx Γ (.cop A B)
+  | case
+      : Stx Γ (.cop A B)
+      → Stx (.mono A :: Γ) C
+      → Stx (.mono B :: Γ) C
+      → Stx Γ C
+
+  | lam : Stx (.mono A :: Γ) B → Stx Γ (.fn A B)
+  | app : Stx Γ (.fn A B) → Stx Γ A → Stx Γ B
+
+  | sing : Stx (dize Γ) T.toTy → Stx Γ (.pow T)
+  | bot : L.Lattice → Stx Γ L
+  | join : L.Lattice → Stx Γ L → Stx Γ L → Stx Γ L
+  | forE : L.Lattice → Stx Γ (.pow T) → Stx (.disc T.toTy :: Γ) L → Stx Γ L
+
+  | discI : Stx (dize Γ) A → Stx Γ (.disc A)
+  | discE : Stx Γ (.disc A) → Stx (.disc A :: Γ) C → Stx Γ C
+
+  | fix : L.Lattice → Stx (.mono L :: dize Γ) L → Stx Γ L
+
+namespace Stx
+
+@[simp]
+theorem sizeOf_cast' {A B As Bs} {a : Stx As A} (h : A = B) (h' : As = Bs)  : sizeOf (cast (by rw [h, h']) a) = sizeOf a := by
+  subst h
+  subst h'
+  rfl
+
+@[simp]
+theorem sizeOf_cast {A B} {a : A} (h : A = B) : sizeOf (cast h a) = sizeOf a := by
+  subst h
+  rfl
+
+def gshift Γ {Γ₁ Γ₂} : Stx (Γ ++ Γ₁) t → Stx (Γ ++ (Γ₂ ++ Γ₁)) t
+  | .var h => .var h.sandwitch_shift
+
+  | .unit => .unit
+  | .prod a b => .prod (gshift _ a) (gshift _ b)
+  | .fst a => .fst (gshift _ a)
+  | .snd a => .snd (gshift _ a)
+
+  | .inl a => .inl (gshift _ a)
+  | .inr a => .inr (gshift _ a)
+  | .case a b c => .case (gshift _ a) (gshift (_ :: _) b) (gshift (_ :: _) c)
+
+  | .lam a => .lam (gshift (_ :: _) a)
+  | .app a b => .app (gshift _ a) (gshift _ b)
+
+  | .sing a =>
+    have := gshift _ (Γ₂ := dize Γ₂) <| cast (by rw [dize_app]) a
+    .sing <| cast (by simp [←dize_app]) this
+  | .bot h => .bot h
+  | .join h a b => .join h (gshift _ a) (gshift _ b)
+  | .forE h a b => .forE h (gshift _ a) (gshift (_ :: _) b)
+
+  | .discI a =>
+    have := gshift _ (Γ₂ := dize Γ₂) <| cast (by rw [dize_app]) a
+    .discI <| cast (by simp [←dize_app]) this
+  | .discE a b => .discE (gshift _ a) (gshift (_ :: _) b)
+
+  | .fix h a =>
+    have := gshift (_ :: _) (Γ₂ := dize Γ₂) <| cast (by rw [dize_app]; rfl) a
+    .fix h <| cast (by simp [←dize_app]) this
+termination_by a => sizeOf a
+decreasing_by
+all_goals simp
+any_goals omega
+all_goals rw [sizeOf_cast']
+any_goals rfl
+any_goals omega
+all_goals simp [dize_app]
+
+/- def parSubst.noopL : {Γ : _} → HList (Stx Γ) (Γ.map ModalType.out) -/
+/-   | [] => .nil -/
+/-   | _ :: _ => .cons (.var .hd) <| noopL.map <| shift [_] -/
+
+end Stx
+
+end DF
