Types/DataFun/Ty.lean
@@ -1,0 +1,96 @@
+
+namespace DF
+
+@[grind]
+inductive FTy where
+  | unit
+  | prod : FTy → FTy → FTy
+  | cop  : FTy → FTy → FTy
+  | pow  : FTy → FTy
+  | disc : FTy → FTy
+
+@[grind]
+inductive Ty where
+  | unit
+  | prod : Ty → Ty → Ty
+  | cop  : Ty → Ty → Ty
+  | fn   : Ty → Ty → Ty
+  | pow  : FTy → Ty
+  | disc : Ty → Ty
+
+@[grind]
+inductive FTy.Lattice : FTy → Prop
+  | unit : Lattice .unit
+  | prod : a.Lattice → b.Lattice → Lattice (.prod a b)
+  | pow : a.Lattice → Lattice (.pow a)
+
+@[grind]
+inductive Ty.Lattice : Ty → Prop
+  | unit : Lattice .unit
+  | prod : a.Lattice → b.Lattice → Lattice (.prod a b)
+  | pow : a.Lattice → Lattice (.pow a)
+
+instance FTy.lDec : {a : FTy} → Decidable a.Lattice
+  | .unit => .isTrue .unit
+  | .prod a b =>
+    match a.lDec, b.lDec with
+    | .isTrue a, .isTrue b => .isTrue <| .prod a b
+    | .isFalse a, _
+    | _, .isFalse _ => .isFalse <| by grind
+  | .pow a =>
+    match a.lDec with
+    | .isTrue a => .isTrue <| .pow a
+    | .isFalse a => .isFalse <| by grind
+  | .cop _ _
+  | .disc _ => .isFalse (by grind)
+
+instance Ty.lDec : {a : Ty} → Decidable a.Lattice
+  | .unit => .isTrue .unit
+  | .prod a b =>
+    match a.lDec, b.lDec with
+    | .isTrue a, .isTrue b => .isTrue <| .prod a b
+    | .isFalse a, _
+    | _, .isFalse _ => .isFalse <| by grind
+  | .pow a =>
+    match a.lDec with
+    | .isTrue a => .isTrue <| .pow a
+    | .isFalse a => .isFalse <| by grind
+  | .fn _ _
+  | .cop _ _
+  | .disc _ => .isFalse (by grind)
+
+def FTy.toTy : FTy → Ty
+  | .unit     => .unit
+  | .cop a b  => .cop a.toTy b.toTy
+  | .prod a b => .prod a.toTy b.toTy
+  | .pow a    => .pow a
+  | .disc a    => .disc a.toTy
+
+inductive ModalType where
+  | disc (t : Ty)
+  | mono (t : Ty)
+
+namespace ModalType
+
+def out : ModalType → Ty | .disc v | .mono v => v
+
+@[grind]
+inductive IsDisc : ModalType → Prop
+  | disc : IsDisc (.disc e)
+
+instance : DecidablePred IsDisc
+  | .disc _ => .isTrue .disc
+  | .mono _ => .isFalse (by grind)
+
+@[grind]
+inductive IsMono : ModalType → Prop
+  | mono : IsMono (.mono e)
+
+instance : DecidablePred IsMono
+  | .disc _ => .isFalse (by grind)
+  | .mono _ => .isTrue .mono
+
+end ModalType
+
+end DF
+
