Types/SysF2/Order.lean
@@ -1,0 +1,11 @@
+import Types.SysF2.Ty
+import Types.SysF2.Stx
+
+def space {n} : Nat → Ty n → Vec Type n → Type
+  | 0, _, _ => Nat
+  | n+1, .fn a b, v => space n a v → space n b v
+  | n+1, .fa a, v => ∀ t, space n a (.cons (space n t v) v)
+  | _+1, .id id, v => v.get id
+
+def obj (t : Ty n) (v : Vec Type n) : Type := ∀ n, space n t v
+
