Types/SysF2/Ty.lean
@@ -1,0 +1,95 @@
+import Mathlib.Tactic.CongrExclamation
+import Types.Utils
+
+inductive Ty : Nat → Type
+  | fn : Ty n → Ty n → Ty n
+  | id : Fin n → Ty n
+  | fa : Ty (n + 1) → Ty n
+
+namespace Ty
+
+def sandwitch (i : Fin (m + k)) : Fin (m + (n + k)) := ⟨i + n, by omega⟩
+
+def gshift k (n : Nat) : Ty (m + k) → Ty (m + (n + k))
+  | .id i => .id <| sandwitch i
+  | .fa (h : Ty (m + (k + 1))) => .fa <| h.gshift _ _
+  | .fn a b => .fn (a.gshift _ n) (b.gshift _ n)
+
+@[simp]
+theorem gshift_0 : {i : Ty (m + k)} → gshift k 0 i = cast (by simp) i
+  | .id ⟨i, h⟩ => by
+    unfold gshift
+    refine eq_of_heq <| (heq_cast_iff_heq _ _ _).mpr ?_
+    congr! <;> simp
+  | .fa h => by
+    unfold gshift
+    refine eq_of_heq <| (heq_cast_iff_heq _ _ _).mpr ?_
+    congr!
+    · simp
+    rw [gshift_0]
+    simp
+  | .fn a b => by
+    unfold gshift
+    refine eq_of_heq <| (heq_cast_iff_heq _ _ _).mpr ?_
+    congr!
+    · simp
+    all_goals rw [gshift_0]
+    all_goals simp
+
+def shift (n : Nat) : Ty m → Ty (m + n) := gshift 0 n
+
+@[simp]
+theorem shift_fn : shift k (.fn a b) = .fn (shift k a) (shift k b) := by
+  simp [shift, gshift]
+
+theorem shift_shift : (v : Ty k)
+    → shift n (shift m v)
+    = cast (congr rfl (Nat.add_assoc _ _ _).symm) (shift _ v)
+  | .id ⟨_,_⟩ => by
+    simp [shift, gshift, sandwitch]
+    sorry
+  | _ => sorry
+
+@[simp]
+theorem shift_0 {i : Ty (m + k)} : shift 0 i = i := by simp [shift]
+
+def subst (hList : Vec (Ty m) n) : Ty n → Ty m
+  | .id i => hList.get i
+  | .fn l r => .fn (l.subst hList) (r.subst hList)
+  | .fa b => .fa
+      <| b.subst
+      <| .cons (.id ⟨0, Nat.zero_lt_succ m⟩)
+      <| hList.map
+      <| shift 1
+
+namespace subst
+
+def noopL : (n : Nat) → Vec (Ty n) n
+  | 0 => .nil
+  | n+1 => .cons (.id 0) <| (noopL n).map <| shift _
+
+@[simp]
+theorem noopL_get : {n : _} → {i : Fin n} → (noopL n).get i = .id i
+  | n+1, ⟨0, _⟩ => by simp [noopL]
+  | n+1, ⟨m+1, _⟩ => by
+    simp only [noopL, Vec.get, Vec.get_map]
+    rw [noopL_get]
+    simp [shift, gshift, sandwitch]
+
+@[simp]
+theorem subst_noopL : {v : _} → subst (noopL n) v = v
+  | .id _ => by simp [subst]
+  | .fa h => by
+    apply (fa.injEq _ _).mpr
+    change subst (noopL _) h = h
+    rw [subst_noopL]
+  | .fn l r => by
+    refine (fn.injEq _ _ _ _).mpr ⟨?_, ?_⟩
+    <;> rw [subst_noopL]
+
+@[simp]
+theorem subst_nil : subst .nil v = v := subst_noopL
+
+end subst
+
+end Ty
