Types/SysFHOAS/Show.lean
@@ -14,15 +14,15 @@ def Type'.show (expr : Type' String) (level : Nat := 0) : String :=
   | .arr t1 t2 => "(" ++ Type'.show t1 level ++ " → " ++ Type'.show t2 level ++ ")"
   | .all  f=> "∀" ++ natToGreek level ++". " ++ Type'.show (f  (natToGreek level)) (level + 1)
 
-def Term'.show {n} {ty : Type'.higher n String}
-    (expr : Term' (T := String) (fun _ _ => String) n ty) (level : Nat := 0) (typelevel : Nat := 0) : String :=
+def Term'.show {ty}
+    (expr : @Term' String (fun _ => String) ty) (level : Nat := 0) (typelevel : Nat := 0) : String :=
   match expr with
   | .var s => s
   | .app t1 t2 => "(" ++ Term'.show t1 level typelevel ++ " " ++ Term'.show t2 level typelevel ++ ")"
   | .lam f => "(λ" ++ natToLetter level ++ "." ++ Term'.show (f (natToLetter level)) (level + 1) typelevel ++ ")"
-  | @Term'.tapp _ _ _ f term1 t => 
-    s!"({Term'.show term1 level typelevel} [{Type'.show (Type'.compress <| f t) typelevel}])"
-  | @Term'.tlam _ _ _ f g => 
-    s!"(Λ {natToGreek typelevel} . {Term'.show (g <| Type'.pvar (natToGreek typelevel)) level (typelevel + 1)})"
+  | @Term'.tapp _ _ f term1 t =>
+    s!"({Term'.show term1 level typelevel} [{Type'.show (Type'.squash <| f t) typelevel}])"
+  | @Term'.tlam _ _ f g =>
+    s!"(Λ {natToGreek typelevel} . {Term'.show (g <| .var (natToGreek typelevel)) level (typelevel + 1)})"
 
 
