Types/SysFHOAS/Stx.lean
@@ -13,19 +13,6 @@ def Type'.squash {rep : Type u} : Type' (Type' rep) → Type' rep
   | .arr a b => .arr a.squash b.squash
   | .all f => .all fun v => (f (.var v)).squash
 
-def Type'.higher (n : Nat) (rep : Type u) := n.succ.repeat Type' rep
-
-def Type'.pvar {n : Nat} {rep} (r : rep) : n.repeat Type' rep :=
-  match n with
-  | 0 => r
-  | _+1 => .var (Type'.pvar r)
-
-def Type'.compress : {n : Nat} → {rep : Type u} → Type'.higher n rep → Type' rep
-  | 0, _, v => v
-  | n+1, _, .var rep => Type'.compress rep
-  | _, _, .arr a b => .arr (Type'.compress a) (Type'.compress b)
-  | _, _, .all f => sorry
-
 def Ty : Type (u + 1) :=  {rep2 : Type u} → Type' rep2
 
 declare_syntax_cat hstx_ty
@@ -46,16 +33,16 @@ macro_rules
   | `([ht| ∀ $i. $v]) => `(Type'.all fun $i => ([ht|$v]))
   | `([ht| ∀ $i $is*. $v]) => `(Type'.all fun $i => ([ht| ∀ $is*. $v]))
 
-inductive Term' {T: Type v} (rep : ∀ n, Type'.higher n T → Type u) : (n : Nat) → Type'.higher n T → Type (max u v) where
-  | var {n t} : rep n t → Term' rep n t
-  | app {n A B} : Term' rep n (Type'.arr A B) → Term' rep n A → Term' rep n B
-  | lam {n A B}: (rep n A → Term' rep n B) → Term' rep n (Type'.arr A B)
-  | tapp {n} : {f : Type'.higher n T → Type'.higher n.succ T}
-    → Term' rep n.succ (Type'.all f)
-    → (t : Type'.higher n T)
-    → Term' rep n (f t).squash
-  | tlam {n f} : ((x : _) → Term' rep n (f x)) → Term' rep n (Type'.all f)
+inductive Term' {T: Type v} (rep : Type' T → Type u) : Type' (Type' T) → Type (max u v) where
+  | var {t} : rep t.squash → Term' rep t
+  | app {A B} : Term' rep (Type'.arr A B) → Term' rep A → Term' rep B
+  | lam {A B}: (rep A.squash → Term' rep B) → Term' rep (Type'.arr A B)
+  | tapp : {f : Type' T → Type' (Type' T)}
+    → Term' rep (Type'.all f)
+    → (t : Type' T)
+    → Term' rep (f t)
+  | tlam {f} : ((x : _) → Term' rep (f x)) → Term' rep (Type'.all f)
 
 def Term (t : Ty) : Type (u + 1) :=
-  {T : Type u} → {n : Nat} → {rep : ∀ n, Type'.higher n T → Type u} → Term' rep n t
+  {T : Type u} → {rep : Type' T → Type u} → Term' rep t
 
